Finished lemma 3

proof.v
@@ -1,211 +1,317 @@
 (* Test *)
 
-Require Import Lists.List.
+Require Import Coq.Init.Datatypes.
+Require Import Coq.Lists.List.
 Require Import Arith.EqNat.
 Require Import Maps.
 
-Definition method := id.
+Fixpoint list_rel { A : Type } (rel : A -> A -> Prop) (l l' : list A) : Prop :=
+  match l, l' with
+  | nil, nil => True
+  | nil, _ => False
+  | _, nil => False
+  | x::xs, y::ys => rel x y /\ list_rel rel xs ys
+  end.
 
-(*
-Inductive lib : Type := .
-Inductive app : Type := .
+Definition var_id := id.
+Definition class_id := id.
+Definition obj_id : class_id := Id 0.
+Inductive var : Type :=
+| Var : var_id -> var
+| This : var.
+Definition field_id := id.
+Definition method_id := id.
+Inductive expr : Type :=
+| E_Var : var -> expr
+| E_Field : expr -> field_id -> expr
+| E_Invk : expr -> method_id -> list expr -> expr
+| E_New : class_id -> list expr -> expr
+| E_Cast : class_id -> expr -> expr.
 
-Inductive class (T : Type) : Type :=
-| Obj : class lib
-| Lib_Clazz : class lib -> list method ->  class lib
-| Ext_Lib : class lib -> list method -> class app
-| Ext_App : class app -> list method -> class app.
+Theorem expr_ind_list :
+  forall P : expr -> Prop,
+       (forall v : var, P (E_Var v)) ->
+       (forall e : expr, P e -> forall f0 : field_id, P (E_Field e f0)) ->
+       (forall e : expr, P e -> forall (m : method_id) (l : list expr), Forall P l -> P (E_Invk e m l)) ->
+       (forall (c : class_id) (l : list expr), Forall P l -> P (E_New c l)) ->
+       (forall (c : class_id) (e : expr), P e -> P (E_Cast c e)) -> forall e : expr, P e.
+  intros P H H0 H1 H2 H3 e. apply expr_rect.
+  - apply H.
+  - apply H0.
+  - admit.
+  - admit.
+  - admit.
+Admitted.
 
-Inductive app_class : Type :=
-| Ext_Lib : lib_class -> list method -> app_class
-| Ext_App : app_class -> list method -> app_class.
- *)
+Definition context := var -> class_id.
 
-(** Definition of class objects which contain their parent class,
-    and class table which just says whether class is in app.
- *)
-Module Rec.
+Definition params := list (class_id * var_id).
+Inductive constr : Type :=
+| Constr : class_id -> params -> list var_id -> list (field_id * var_id) -> constr.
+Inductive method := Method : class_id -> method_id -> params -> expr -> method.
 
-  Inductive class : Type :=
-  | Obj : class
-  | C : class -> list method -> class.
+Inductive class : Type :=
+| Obj : class
+| C : class_id -> class_id -> list (class_id * field_id) -> constr -> list method -> class.
 
-  Inductive class_table : Type :=
-  | CT : (class -> Prop) -> class_table.
-
-  Definition in_app (ct : class_table) (c : class) : Prop :=
-    match ct with
-    | CT f => f c
-    end.
-
-End Rec.
-
-Module ParId.
-
-  Inductive class : Type :=
-  | Obj : class
-  | C : id -> list method -> class.
-
-  Definition class_table : Type := partial_map class * partial_map class.
-
-  Definition extends_id (ct : class_table) (i : id) (d : class) : Prop :=
-    match ct with (app, lib) => app i = Some d \/ lib i = Some d end.
-
-  Definition extends (ct : class_table) (c d : class) : Prop :=
-    match c with
-    | Obj => False
-    | C i _ => extends_id ct i d
-    end.
+Definition class_table : Type := partial_map class * partial_map class.
 
 
-  Definition in_lib_id (ct : class_table) (i : id) : Prop :=
-    match ct with (_, lib) => lib i <> None end.
+Definition lookup (ct : class_table) (i : class_id) : option class :=
+  match ct with (app, lib) =>
+                match app i with
+                | Some c => Some c
+                | None => lib i
+                end
+  end.
+Definition lookup_field (c : class) (f : field_id) : option class_id :=
+  match c with
+  | Obj => None
+  | C _ _ fs _ _ => match find (fun fp => beq_id (snd fp) f) fs with
+                   | None => None
+                   | Some (ci, _) => Some ci
+                   end
+  end.
+Definition lookup_method (c : class) (mi : method_id) : option method :=
+  match c with
+  | Obj => None
+  | C _ _ _ _ ms => find (fun m => match m with Method _ mi' _ _ => beq_id mi mi' end) ms
+  end.
+Definition id_of (c : class) : class_id :=
+  match c with
+  | Obj => obj_id
+  | C ci _ _ _ _ => ci
+  end.
 
-  Definition in_app_id (ct : class_table) (i : id) : Prop :=
-    match ct with (app, _) => app i <> None end.
+Definition par_id_of (c : class) : option class_id :=
+  match c with
+  | Obj => None
+  | C _ di _ _ _ => Some di
+  end.
 
-  Definition in_table_id (ct : class_table) (i : id) : Prop :=
-    in_lib_id ct i \/ in_app_id ct i.
+Definition in_lib_id (ct : class_table) (i : class_id) : Prop :=
+  match ct with (_, lib) => lib i <> None end.
+                
+Definition in_app_id (ct : class_table) (i : class_id) : Prop :=
+  match ct with (app, _) => app i <> None end.
 
-  Definition in_lib (ct : class_table) (c : class) : Prop :=
-    match c with
-    | Obj => True
-    | C i _ => in_lib_id ct i
-    end.
-  Definition in_app (ct : class_table) (c : class) : Prop :=
-    match c with
-    | Obj => False
-    | C i _ => in_app_id ct i
-    end.
-  Definition in_table (ct : class_table) (c : class) : Prop :=
-    match c with
-    | Obj => True
-    | C i _ => in_table_id ct i
-    end.
-  Lemma in_table_app_or_lib : forall (ct : class_table) (c : class),
-      in_table ct c <-> in_lib ct c \/ in_app ct c.
-  Proof.
-    intros. destruct c.
-    - simpl. split. auto. auto. 
-    - unfold in_table, in_lib, in_app. unfold in_table_id. reflexivity.
-  Qed.
-  Lemma in_app_in_table : forall (ct : class_table) (c : class),
-      in_app ct c -> in_table ct c.
-  Proof. intros. rewrite in_table_app_or_lib. right. apply H. Qed.
-  Lemma in_lib_in_table : forall (ct : class_table) (c : class),
-      in_lib ct c -> in_table ct c.
-  Proof. intros. rewrite in_table_app_or_lib. left. apply H. Qed.
+Definition in_lib (ct : class_table) (c : class) : Prop :=
+  match ct with (_, lib) => lib (id_of c) <> None end.
+                
+Definition in_app (ct : class_table) (c : class) : Prop :=
+  match ct with (app, _) => app (id_of c) <> None end.
+
+Definition in_table_id (ct : class_table) (i : class_id) : Prop :=
+  in_app_id ct i \/ in_lib_id ct i.
+
+Definition in_table (ct : class_table) (c : class) : Prop :=
+  in_app ct c \/ in_lib ct c.
+
+Lemma in_app_in_table : forall (ct : class_table) (c : class),
+    in_app ct c -> in_table ct c.
+Proof. intros. unfold in_table. left. apply H. Qed.
+Lemma in_lib_in_table : forall (ct : class_table) (c : class),
+    in_lib ct c -> in_table ct c.
+Proof. intros. unfold in_table. right. apply H. Qed.
+
+Definition extends (ct : class_table) (c d : class) : Prop :=
+  match c with
+  | Obj => False
+  | C _ di _ _ _ => lookup ct di = Some d
+  end.
+
+Definition extends_id (ct : class_table) (ci di : class_id) : Prop :=
+  match lookup ct ci with
+  | None => False
+  | Some Obj => False
+  | Some (C _ di' _ _ _) => di = di'
+  end.
+
+Inductive subtype (ct : class_table) : class -> class -> Prop :=
+| S_Ref : forall (c : class), subtype ct c c
+| S_Trans : forall (c d e : class), subtype ct c d -> subtype ct d e -> subtype ct c e
+| S_Sub : forall (c d : class), extends ct c d -> subtype ct c d.
+
+Inductive subtype_id (ct : class_table) : class_id -> class_id -> Prop :=
+| SI_Ref : forall ci, in_table_id ct ci -> subtype_id ct ci ci
+| SI_Sub : forall ci di, extends_id ct ci di -> subtype_id ct ci di
+| SI_Trans : forall ci di ei, subtype_id ct ci di -> subtype_id ct di ei -> subtype_id ct ci ei.
+
+Inductive valid_class (ct : class_table) : class -> Type :=
+| ValidObj : in_lib ct Obj -> ~ in_app ct Obj -> lookup ct obj_id = Some Obj -> valid_class ct Obj
+| ValidParent : forall c d,
+    valid_class ct d -> extends ct c d ->
+    ~ (in_lib ct c /\ in_app ct c) ->
+    (in_lib ct d /\ in_table ct c) \/ (in_app ct d /\ in_app ct c)  ->
+    lookup ct (id_of c) = Some c ->
+    valid_class ct c.
+
+Fixpoint mtype (ct : class_table) (mi : method_id) (c : class) (pfc : valid_class ct c) :
+  option (list class_id * class_id) :=
+  match pfc with
+  | ValidObj _ _ _ _ => None
+  | ValidParent _ d pfd _ _ _ _ _ =>
+    match lookup_method c mi with
+    | None => None
+    | Some (Method ci _ l_arg _) => Some (map fst l_arg, ci) 
+    end
+  end.
+
+Fixpoint fields (ct : class_table) (c : class) (pfc : valid_class ct c) : list class_id :=
+  match pfc, c with
+  | ValidObj _ _ _ _, _ => nil
+  | ValidParent _ _ d pfd _ _ _ _ , C _ _ fs _ _ => map fst fs ++ fields ct d pfd
+  | _, _ => nil
+  end.
+
+Inductive type_of (ct : class_table) (gamma : context) : expr -> class_id -> Prop :=
+| T_Var : forall x, type_of ct gamma (E_Var x) (gamma x)
+| T_Field : forall e c di f,
+    type_of ct gamma e (id_of c) -> lookup_field c f = Some di ->
+    type_of ct gamma (E_Field e f) di
+| T_Invk : forall e0 c0 ci0 pfc0 ld ret mi le lc,
+    id_of c0 = ci0 -> type_of ct gamma e0 ci0 -> mtype ct mi c0 pfc0 = Some (ld, ret) ->
+    length ld = length le -> length le = length lc ->
+    Forall (fun p => type_of ct gamma (fst p) (snd p)) (combine le lc) ->
+    Forall (fun p => subtype_id ct (fst p) (snd p)) (combine lc ld) ->
+    type_of ct gamma (E_Invk e0 mi le) ci0
+| T_New : forall c ci pfc le lc ld,
+    id_of c = ci -> fields ct c pfc = ld ->
+    length ld = length le -> length le = length lc ->
+    Forall (fun p => type_of ct gamma (fst p) (snd p)) (combine le lc) ->
+    Forall (fun p => subtype_id ct (fst p) (snd p)) (combine lc ld) ->
+    type_of ct gamma (E_New ci le) ci
+| T_Cast : forall e0 ci di, type_of ct gamma e0 di -> type_of ct gamma (E_Cast ci e0) ci.
+
+Inductive type_checks (ct : class_table) (gamma : context) : expr -> Prop :=
+| TC_Var : forall x, in_table_id ct (gamma x) -> type_checks ct gamma (E_Var x)
+| TC_Field : forall e f di, type_of ct gamma (E_Field e f) di -> in_table_id ct di -> type_checks ct gamma e ->
+                       type_checks ct gamma (E_Field e f)
+| TC_Invk : forall e m le di, type_of ct gamma (E_Invk e m le) di -> in_table_id ct di ->
+                      type_checks ct gamma e -> Forall (type_checks ct gamma) le ->
+                      type_checks ct gamma (E_Invk e m le)
+| TC_New : forall ci le, in_table_id ct ci -> Forall (type_checks ct gamma) le -> type_checks ct gamma (E_New ci le)
+| TC_Cast : forall e di, in_table_id ct di -> type_checks ct gamma e -> type_checks ct gamma (E_Cast di e).
+(*  exists c, type_of ct gamma e c /\ in_table_id ct c. *)
+
   
-  Inductive valid_class (ct : class_table) : class -> Type :=
-  | ValidObj : valid_class ct Obj
-  | ValidParent : forall i ms d,
-      valid_class ct d -> extends ct (C i ms) d ->
-      ~ (in_lib ct (C i ms) /\ in_app ct (C i ms)) ->
-      (in_lib ct d /\ in_table ct (C i ms)) \/ (in_app ct d /\ in_app ct (C i ms))  ->
-      valid_class ct (C i ms).
-        
+Definition valid_table (ct : class_table) : Type :=
+  forall c, in_table ct c -> valid_class ct c.
 
-  Definition valid_table (ct : class_table) : Type :=
-    forall c, in_table ct c -> valid_class ct c.
+Lemma extends_injective : forall ct c d d',
+    valid_class ct c -> extends ct c d -> extends ct c d' -> d = d'.
+Proof.
+  intros ct c d d' pfc c_ext_d c_ext_d'.
+  unfold extends in c_ext_d, c_ext_d'. destruct c as [| ci di k ms fs].
+  - inversion c_ext_d.
+  - rewrite c_ext_d in c_ext_d'. inversion c_ext_d'. reflexivity.
+Qed.
 
-  Lemma extends_injective : forall ct c d d',
-      valid_class ct c -> extends ct c d -> extends ct c d' -> d = d'.
-  Proof.
-    intros ct c d d' pfc c_ext_d c_ext_d'.
-    unfold extends in c_ext_d, c_ext_d'. destruct c as [| i ms].
-    - inversion c_ext_d.
-    - unfold extends_id in c_ext_d, c_ext_d'. remember ct as ct'. destruct ct' as [app lib]. inversion pfc.
-      destruct c_ext_d as [d_in_app | d_in_lib], c_ext_d' as [d'_in_app | d'_in_lib].
-      + rewrite d_in_app in d'_in_app. inversion d'_in_app. reflexivity.
-      + assert (in_lib (app, lib) (C i ms)) as c_in_lib.
-        { unfold in_lib, in_lib_id, not. intros. rewrite d'_in_lib in H5. inversion H5. }
-        assert (in_app (app, lib) (C i ms)) as c_in_app.
-        { unfold in_app, in_app_id, not. intros. rewrite d_in_app in H5. inversion H5. }
-        unfold not in H3. assert False. apply H3. split. apply c_in_lib. apply c_in_app. inversion H5.
-      + assert (in_lib (app, lib) (C i ms)) as c_in_lib.
-        { unfold in_lib, in_lib_id, not. intros. rewrite d_in_lib in H5. inversion H5. }
-        assert (in_app (app, lib) (C i ms)) as c_in_app.
-        { unfold in_app, in_app_id, not. intros. rewrite d'_in_app in H5. inversion H5. }
-        unfold not in H3. assert False. apply H3. split. apply c_in_lib. apply c_in_app. inversion H5.
-      + rewrite d_in_lib in d'_in_lib. inversion d'_in_lib. reflexivity.
-  Qed.
-        
+Definition dmethods (c : class) : list method_id :=
+  match c with
+  | Obj => nil
+  | C _ _ _ _ ms => map (fun m => match m with Method _ id _ _ => id end) ms
+  end.
 
-  Fixpoint mresolve (ct : class_table) (m : method) (c : class) (pfc : valid_class ct c) : option class :=
-    match pfc with
-    | ValidObj _ => None
-    | ValidParent _ _ ms d pfd _ _ _  => if (existsb (fun m' => beq_id m m') ms)
-                                        then Some c
-                                        else mresolve ct m d pfd
-    end.
+Fixpoint mresolve (ct : class_table) (m : method_id) (c : class) (pfc : valid_class ct c) : option class :=
+  match pfc with
+  | ValidObj _ _ _ _ => None
+  | ValidParent _ _ d pfd _ _ _ _ => if (existsb (fun m' => beq_id m m') (dmethods c))
+                                      then Some c
+                                      else mresolve ct m d pfd
+  end.
 
-  Lemma mres_lib_in_lib : forall (ct : class_table) (m : method) (c e : class) (pfc : valid_class ct c),
-      in_lib ct c -> mresolve ct m c pfc = Some e -> in_lib ct e.
-    admit.
-  Admitted.
-  Lemma lemma1 : forall (ct : class_table) (c e : class) (m : method) (pfc : valid_class ct c),
-      mresolve ct m c pfc = Some e -> in_app ct e -> in_app ct c.
-  Proof.
-    intros. induction pfc.
-    - unfold mresolve in H. inversion H.
-    - unfold mresolve in H. destruct (existsb (fun m' : id => beq_id m m') ms) in H.
-      + inversion H. rewrite H2. apply H0.
-      + fold mresolve in H. apply IHpfc in H. destruct o.
-        * inversion pfc.
-          -- rewrite <- H2 in H. unfold in_app in H. inversion H.
-          -- rewrite H6 in H4. destruct H4. split. destruct H1. apply H1. apply H.
-        * destruct H1. apply H2.
-  Qed.
+Lemma mres_lib_in_lib : forall (ct : class_table) (m : method_id) (c e : class) (pfc : valid_class ct c),
+    in_lib ct c -> mresolve ct m c pfc = Some e -> in_lib ct e.
+  intros ct m c e pfc c_in_lib c_res_e.
+  induction pfc.
+  - inversion c_res_e.
+  - unfold mresolve in c_res_e. destruct (existsb (fun m' : id => beq_id m m') (dmethods c)) in c_res_e.
+    + inversion c_res_e. rewrite <- H0. apply c_in_lib.
+    + fold mresolve in c_res_e. apply IHpfc.
+      * destruct o.
+        -- destruct H. apply H.
+        -- destruct n. split. apply c_in_lib. destruct H. apply H0.
+      * apply c_res_e.
+Qed.
 
-  Inductive ave_rel (ct ct' : class_table) : Prop :=
-    | AveRel :  valid_table ct -> valid_table ct' ->
-                (forall c, in_app ct c <-> in_app ct' c) ->
-                (forall c d, extends ct c d -> in_table ct' c -> extends ct' c d) ->
-                (forall c d, extends ct c d -> in_lib ct d -> in_table ct' c -> in_lib ct' d) ->
-                ave_rel ct ct'.
+Inductive ave_rel (ct ct' : class_table) : Prop :=
+  | AveRel :  valid_table ct -> valid_table ct' ->
+              (forall c, in_app ct c <-> in_app ct' c) ->
+              (forall c d, extends ct c d -> in_table ct' c -> extends ct' c d) ->
+              (forall c d, extends ct c d -> in_lib ct d -> in_table ct' c -> in_lib ct' d) ->
+              ave_rel ct ct'.
 
-  Lemma lib'_subset_lib : forall (ct ct' : class_table) (c : class),
-      ave_rel ct ct' -> in_table ct' c -> in_lib ct c -> in_lib ct' c.
-  Proof.
-    intros. inversion H. rewrite in_table_app_or_lib in H0. destruct H0.
-    - apply H0.
-    - apply H2 in H0. unfold valid_table in X.
-      assert (in_table ct c). { apply in_app_in_table. apply H0. }
-      apply X in H5. inversion H5.
-      + rewrite <- H6 in H0. inversion H0.
-      + rewrite H10 in H8. destruct H8. split. apply H1. apply H0.
-  Qed.
+Lemma lib'_subset_lib : forall (ct ct' : class_table) (c : class),
+    ave_rel ct ct' -> in_table ct' c -> in_lib ct c -> in_lib ct' c.
+Proof.
+  intros. inversion H. unfold in_table in H0. destruct H0.
+  - apply H2 in H0. unfold valid_table in X.
+    assert (in_table ct c). { apply in_app_in_table. apply H0. }
+    apply X in H5. inversion H5.
+    + rewrite <- H9 in H0. unfold not in H7. apply H7 in H0. inversion H0.
+    + destruct H8. split. apply H1. apply H0. 
+  - apply H0.
+Qed.
 
-  (*Lemma ext_in_ct_ext_in_ct' : forall (ct ct' : class_table) (c d : class),
-      ave_rel ct ct' -> in_table ct c -> in_table ct' c -> extends ct c d -> extends ct' c d.
-  Proof.
-    intros ct ct' c d ave cin cin' ext.*)
-    
-    
+Inductive alpha (ct ct' : class_table) (pft : ave_rel ct ct') : expr * expr -> Prop :=
+| Rel_Field : forall e e' f, alpha ct ct' pft (e, e') -> alpha ct ct' pft (E_Field e f, E_Field e' f)
+| Rel_Invk : forall e e' le le' m, alpha ct ct' pft (e, e') -> length le = length le' -> Forall (alpha ct ct' pft) (combine le le') ->
+                              alpha ct ct' pft (E_Invk e m le, E_Invk e' m le')
+| Rel_New : forall ci le le', in_table_id ct' ci -> length le = length le' ->
+                         Forall (alpha ct ct' pft) (combine le le') ->
+                         alpha ct ct' pft (E_New ci le, E_New ci le')
+| Rel_Cast : forall e e' c, alpha ct ct' pft (e, e') -> alpha ct ct' pft (E_Cast c e, E_Cast c e').
 
-  Lemma lemma2 : forall (ct ct' : class_table) (c e e' : class) (m : method) (pfc : valid_class ct c) (pfc' : valid_class ct' c),
-      in_app ct c -> mresolve ct m c pfc = Some e -> mresolve ct' m c pfc' = Some e'  -> ave_rel ct ct' ->
-      in_app ct e \/ in_lib ct' e'.
+Definition subst := var -> expr.
+
+Fixpoint do_sub (sig : subst) (e : expr) : expr :=
+ match e with
+ | E_Var v => sig v
+ | E_Field e' f => E_Field (do_sub sig e') f
+ | E_Invk e' m es => E_Invk (do_sub sig e') m (map (do_sub sig) es)
+ | E_New c es => E_New c (map (do_sub sig) es)
+ | E_Cast c e' => E_Cast c (do_sub sig e')
+ end.
+
+Lemma lemma1 : forall (ct : class_table) (c e : class) (m : method_id) (pfc : valid_class ct c),
+    mresolve ct m c pfc = Some e -> in_app ct e -> in_app ct c.
+Proof.
+  intros ct c e m pfc c_res_e e_in_app. induction pfc as [ | c d pfd IHd c_ext_d not_lib_app sca look].
+  - unfold mresolve in c_res_e. inversion c_res_e.
+  - unfold mresolve in c_res_e. destruct (existsb (fun m' : id => beq_id m m') (dmethods c)) in c_res_e.
+    + inversion c_res_e. apply e_in_app.
+    + fold mresolve in c_res_e. apply IHd in c_res_e. destruct sca.
+      * inversion pfd.
+        -- rewrite <- H3 in c_res_e. unfold not in H1. apply H1 in c_res_e. inversion c_res_e.
+        -- destruct H2. split. destruct H. apply H. apply c_res_e.
+      * destruct H. apply H0.
+Qed.
+
+Lemma lemma2 : forall (ct ct' : class_table) (c e e' : class) (m : method_id)
+                 (pfc : valid_class ct c) (pfc' : valid_class ct' c),
+    in_app ct c -> mresolve ct m c pfc = Some e -> mresolve ct' m c pfc' = Some e'  -> ave_rel ct ct' ->
+    in_app ct e \/ in_lib ct' e'.
 Proof.
   intros ct ct' c e e' m pfc pfc' c_in_app c_res_e c_res_e' rel.
-  induction pfc as [| i ms d pfd IHd c_ext_d not_lib_app app_ext_app].
+  induction pfc as [| c d pfd IHd c_ext_d not_lib_app app_ext_app].
   (* c is Obj *)
   - unfold mresolve in c_res_e. inversion c_res_e.
   (* c extends d *)
-  - unfold mresolve in c_res_e. fold mresolve in c_res_e.
-    destruct (existsb (fun m' : id => beq_id m m') ms) eqn:m_res.
+  - unfold mresolve in c_res_e; fold mresolve in c_res_e.
+    destruct (existsb (fun m' : id => beq_id m m') (dmethods c)) eqn:m_res.
     (* m-res *)
-    + inversion c_res_e. left. apply c_in_app.
+    + inversion c_res_e; left; rewrite <- H0; eauto. 
     (* m-res-inh *)
     + inversion rel as [ct_val ct'_val keep_app keep_ext keep_lib].
-      remember (C i ms) as c. unfold mresolve in c_res_e'.
-      (* can't induct on pfc and pfc' simultaneously, so manually destruct pfc' and show that it's the same d *)
-      destruct pfc' as [_ | i0 ms0 d0 pfd' c_ext_d'] eqn:pfc''.
+      unfold mresolve in c_res_e'.
+      (* can't induct on pfc and pfc' simultaneously,
+         so manually destruct pfc' and show that it's the same parent *)
+      destruct pfc' as [| c0 d0 pfd' c_ext_d'] eqn:pfc''.
       * inversion c_res_e'.
-      * fold mresolve in c_res_e'. inversion Heqc.
-        rewrite H1 in c_res_e'. rewrite m_res in c_res_e'.
+      * fold mresolve in c_res_e'. rewrite m_res in c_res_e'.
         assert (d = d0) as deq.
-        { apply extends_injective with (ct := ct') (c := (C i0 ms0)).
+        { apply extends_injective with (ct := ct') (c := c0).
           -- apply pfc'.
           -- apply keep_ext.
              ++ apply c_ext_d.
@@ -214,7 +320,7 @@ Proof.
         destruct app_ext_app as [[d_in_lib _] | [d_in_app _]].
         (* d in lib - use averroes transformation properties *)
         -- right. apply mres_lib_in_lib with (m := m) (c := d0) (pfc := pfd').
-           ++ apply keep_lib with (c := (C i0 ms0)).
+           ++ apply keep_lib with (c := c0).
               ** rewrite <- deq. apply c_ext_d.
               ** rewrite <- deq. apply d_in_lib.
               ** apply in_app_in_table. apply keep_app. apply c_in_app.
@@ -225,138 +331,33 @@ Proof.
                       mresolve ct' m d pfc' = Some e' -> in_app ct e \/ in_lib ct' e') as IHd'.
            { intros pfc'0 _ mres'. apply IHd with (pfc' := pfc'0).
              apply d_in_app. apply c_res_e. apply mres'. }
-           rewrite deq in IHd'. 
+           rewrite deq in IHd'.
            apply IHd' with (pfc' := pfd').
            ++ rewrite <- deq. apply d_in_app.
            ++ apply c_res_e'.
 Qed.
-         
-       
-End ParId.
 
-Module ParC.
+(* Lemma Forall_imp : forall (A : type) (l : list A)  *)
 
-  Inductive class : Type :=
-  | Obj : class
-  | C : class -> list method -> class.
-
-  (** application classes * library classes  *)
-  Definition class_table : Type := list class * list class.
-
-  Definition in_table (ct : class_table) (c : class) : Prop :=
-    match ct with (app, lib) => In c app \/ In c lib end.
-
-  Definition in_app (ct : class_table) (c : class) : Prop :=
-    match ct with (app, _) => In c app end.
-
-  Definition in_lib (ct : class_table) (c : class) : Prop :=
-    match ct with (_, lib) => In c lib end.
-
-  Inductive valid_class (ct : class_table) : class -> Type :=
-  | ValidObj : valid_class ct Obj
-  | ValidParent : forall c ms,
-      valid_class ct c ->
-      ~ (in_lib ct (C c ms) /\ in_app ct (C c ms)) ->
-      (in_lib ct c /\ in_table ct (C c ms)) \/ (in_app ct c /\ in_app ct (C c ms))  ->
-      valid_class ct (C c ms).
-
-  Definition extends (c d : class) : Prop :=
-    match c with
-    | Obj => False
-    | C c' _ => c' = d
-    end.
-
-  Definition valid_table (ct : class_table) : Type :=
-    match ct with
-    | (app, lib) => forall c, in_table ct c -> valid_class ct c
-    end.
-
-  Fixpoint mresolve (m : method) (c : class) : option class :=
-    match c with
-    | Obj => None
-    | C d ms => if (existsb (fun m' => beq_id m m') ms) then Some c else mresolve m d
-    end.
-  
-  Lemma lemma1 : forall (ct : class_table) (pft : valid_table ct) (c e : class) (pfc : valid_class ct c) (pfe : valid_class ct e) (m : method),
-      mresolve m c = Some e -> in_app ct e -> in_app ct c.
-  Proof.
-    intros. induction pfc.
-    - unfold mresolve in H. inversion H.
-    - unfold mresolve in H. destruct (existsb (fun m' : id => beq_id m m') ms) in H.
-      + inversion H. rewrite H2. apply H0.
-      + fold mresolve in H. apply IHpfc in H. destruct o.
-        * destruct n. destruct H1. split. apply H1. apply H.
-        * destruct H1. apply H2.
-  Qed.
-  
-End ParC.
-(*
-Definition extends (c d : class) : Prop :=
-  match c with
-  | Obj => False
-  | C d' ms => d' = d
-  end.
-
-Definition parent (c : class) : class :=
-  match c with
-  | Obj => Obj
-  | C d _ => d
-  end.
-*)
-Axiom obj_in_lib : forall (ct : class_table), ~ (in_app ct Obj).
-
-Axiom no_lib_ext_app : forall (ct : class_table) (c : class) (ms : list method),
-    in_app ct c -> in_app ct (C c ms).
-
-Module NonInductive.
-  Fixpoint mresolve (ct : class_table) (m : method) (c : class) : class :=
-    match c with
-    | Obj => Obj
-    | C d ms => if (existsb (fun m' => beq_id m m') ms) then c else mresolve ct m d
-    end.
-  
-  Lemma lemma1 : forall (ct : class_table) (c : class) (m : method),
-      in_app ct (mresolve ct m c) -> in_app ct c.
-  Proof.
-    intros. induction c as [| d ms].
-    - simpl in H. apply obj_in_lib in H. inversion H.
-    - simpl in H. destruct (existsb (fun m' : id => beq_id m m') l) in H.
-      + apply H.
-      + apply ms in H. apply no_lib_ext_app. apply H.
-  Qed.
-  
-End NonInductive.
-
-Module Induct.
-  Inductive mresolve (ct : class_table) : method -> class -> class -> Prop :=
-  | Mres : forall (m : method) (c : class) (ms : list method),
-      In m ms -> mresolve ct m (C c ms) (C c ms)
-  | Mres_Inh : forall (m : method) (c d : class) (ms : list method),
-      ~ In m ms -> mresolve ct m c d -> mresolve ct m (C c ms) d.
-
-  Lemma lemma1 : forall (ct : class_table) (c d : class) (m : method),
-      mresolve ct m c d -> in_app ct d -> in_app ct c.
-  Proof.
-    intros. induction H.
-    - (* Mres *) apply H0.
-    - (* Mres-Inh *) apply no_lib_ext_app. auto. 
-  Qed.
-End Induct.
-
-Module InductOpt.
-  Inductive mresolve (ct : class_table) : method -> class -> option class -> Prop :=
-  | M_Res_None : forall (m : method), mresolve ct m Obj None
-  | M_Res : forall (m : method) (c : class) (ms : list method),
-    In m ms -> mresolve ct m (C c ms) (Some (C c ms))
-  | M_Res_Inh : forall (m : method) (c : class) (d : option class) (ms : list method),
-    ~ In m ms -> mresolve ct m c d -> mresolve ct m (C c ms) d.
-
-Lemma lemma1 : forall (ct : class_table) (c d : class) (m : method),
-    mresolve ct m c (Some d) -> in_app ct d -> in_app ct c.
+Lemma lemma3 : forall (ct ct' : class_table) (pft : ave_rel ct ct')
+                 (sig sig' : subst) (gamma : context) (e0 : expr),
+    (forall v, alpha ct ct' pft (sig v, sig' v)) -> type_checks ct' gamma e0 ->
+    alpha ct ct' pft (do_sub sig e0, do_sub sig' e0).
 Proof.
-  intros. remember (Some d) as sd. induction H.
-  - (* Obj *) inversion Heqsd.
-  - (* Mres *) inversion Heqsd. rewrite <- H2 in H0. apply H0.
-  - (* Mres-Inh *) apply IHmresolve in Heqsd. apply no_lib_ext_app. apply Heqsd.
+  intros ct ct' pft sig sig' gamma e0 rel typ_chk. induction e0 using expr_ind_list.
+  - eauto.
+  - simpl; apply Rel_Field. inversion typ_chk; eauto. 
+  - simpl; apply Rel_Invk.
+    + inversion typ_chk; eauto. 
+    + rewrite map_length, map_length; reflexivity.
+    + inversion typ_chk. clear H2; clear H3; clear typ_chk; induction l.
+      * apply Forall_nil. 
+      * inversion H; inversion H6. apply Forall_cons; eauto; eauto.
+  - simpl. inversion typ_chk. apply Rel_New.
+    + eauto.
+    + rewrite map_length, map_length; reflexivity.
+    + clear typ_chk; clear H1; induction l.
+      * apply Forall_nil.
+      * inversion H; inversion H3. apply Forall_cons; eauto; eauto.
+  - apply Rel_Cast; inversion typ_chk; eauto.
 Qed.
-End InductOpt.
